Cannonical forms lemma done

SystemFD/Metatheory/Cannonicity.lean
@@ -93,8 +93,6 @@ cases tJ; case _ wf h1 =>
     exfalso
     apply datatype_opent_distinct vctor vit
 
-
-
 theorem cannonical_insttype_head :
   Γ ⊢ #h : T ->
   Γ ⊢ T : ★ ->
@@ -134,3 +132,207 @@ cases tJ; case _ wf h1 =>
   case _ =>
     injection h1 with h1; cases h1;
     simp; rw [fh]; unfold Frame.is_insttype; simp;
+
+inductive ArrowLike  : (T : Term) -> Prop where
+  | arrowt : ArrowLike (A -t> B)
+  | allt : ArrowLike (∀[A] B)
+
+inductive LambdaLike : (T : Term) -> Prop where
+  | lam : LambdaLike (`λ[A] B)
+  | lamt : LambdaLike (Λ[A] B)
+
+@[simp]
+abbrev CannonicalLambdaType (Γ : Ctx Term) : (v : JudgmentVariant) -> JudgmentArgs v -> Prop
+| .prf => λ (t, τ) =>
+       Val Γ t ->
+       Γ ⊢ t : τ ->
+       Γ ⊢ τ : ★ ->
+       ArrowLike τ ->
+       ((LambdaLike t) ∨ (ValidHeadVariable t Γ.is_ctor ∨ ValidHeadVariable t Γ.is_insttype))
+| .wf => λ () => true
+
+theorem cannonical_lambda :
+  Judgment v Γ idx ->
+  CannonicalLambdaType Γ v idx
+  := by
+intro j; induction j <;> simp at *
+all_goals (intro h1 h2 h3 h4)
+any_goals try (solve | cases h1; case _ h1 => cases h1)
+any_goals try (solve | cases h3)
+case _ Γ n T wf gt ih =>
+  cases h1; case _ n_stable nnf =>
+  simp at nnf; cases nnf; case _ e1 e2 =>
+  subst e1; subst e2;
+  generalize fh : Γ d@ n = f at *;
+  unfold Frame.get_type at gt;
+  cases h4;
+  case _ =>
+    split at gt;
+    any_goals (solve | cases gt)
+    any_goals (solve | unfold Ctx.is_stable_red at n_stable; unfold Frame.is_stable_red at n_stable;
+                       exfalso; rw[fh] at n_stable; simp at n_stable)
+    all_goals (cases gt)
+    case _ =>
+      have lem := classification_lemma h3; simp at lem;
+      cases lem;
+      case _ =>
+        have wfr := @frame_wf_by_index Γ n wf;
+        have h := ctx_get_var_type wf fh;
+        cases h
+      case _ h =>
+        cases h; case _ k h => cases h; case _ _ h => cases h; case _ h => cases h
+    case _ =>
+      have wfr := @frame_wf_by_index Γ n wf;
+      have h := ctx_get_datatype_kind wf fh;
+      cases h;
+    case _ =>
+      apply Or.inr; apply Or.inl; unfold ValidHeadVariable;
+      apply Exists.intro (n, []);
+      apply And.intro; simp; simp; rw[fh]; unfold Frame.is_ctor; simp
+    case _ =>
+      have wfr := @frame_wf_by_index Γ n wf;
+      have h := ctx_get_opent_kind wf fh;
+      cases h;
+    case _ =>
+      apply Or.inr; apply Or.inr; unfold ValidHeadVariable;
+      apply Exists.intro (n, []);
+      apply And.intro; simp; simp; rw[fh]; unfold Frame.is_insttype; simp
+  case _ =>
+    split at gt;
+    any_goals (solve | cases gt)
+    any_goals (solve | unfold Ctx.is_stable_red at n_stable; unfold Frame.is_stable_red at n_stable;
+                       exfalso; rw[fh] at n_stable; simp at n_stable)
+    all_goals (cases gt)
+    case _ =>
+      have lem := classification_lemma h3; simp at lem;
+      cases lem;
+      case _ =>
+        have wfr := @frame_wf_by_index Γ n wf;
+        have h := ctx_get_var_type wf fh;
+        cases h
+      case _ h =>
+        cases h; case _ k h => cases h; case _ _ h => cases h; case _ h => cases h
+    case _ =>
+      have wfr := @frame_wf_by_index Γ n wf;
+      have h := ctx_get_datatype_kind wf fh;
+      cases h;
+    case _ =>
+      apply Or.inr; apply Or.inl; unfold ValidHeadVariable;
+      apply Exists.intro (n, []);
+      apply And.intro; simp; simp; rw[fh]; unfold Frame.is_ctor; simp
+    case _ =>
+      have wfr := @frame_wf_by_index Γ n wf;
+      have h := ctx_get_opent_kind wf fh;
+      cases h;
+    case _ =>
+      apply Or.inr; apply Or.inr; unfold ValidHeadVariable;
+      apply Exists.intro (n, []);
+      apply And.intro; simp; simp; rw[fh]; unfold Frame.is_insttype; simp
+
+case _ Γ f _ _ _ fJ _ _ ih => -- appk bogus case
+  cases h1; case _ n ts n_stable ts' =>
+  simp at ts'; rw [Option.bind_eq_some] at ts';  cases ts'; case _ w fnf =>
+  cases fnf; case _ fnf ts' =>
+  cases ts';
+  have vf : Val Γ f := by constructor; assumption; assumption
+  generalize fh : Γ d@ w.fst = f at *;
+  have lem := classification_lemma fJ; simp at lem; cases lem;
+  case _ h => cases h; case _ k1 k2 =>
+    have h := uniqueness_of_types h3 k2; cases h;
+  case _ h =>
+    cases h; case _ w h =>
+    cases h; case _ wk arrk =>
+    cases arrk; cases wk;
+
+case lam Γ A t B ih1 ih2 =>  constructor; constructor
+
+case app Γ f A B a B' fJ aJ h0 ih1 ih2 =>
+  cases h1; case _ n ts n_stable h1 =>
+  simp at h1; rw[Option.bind_eq_some] at h1;
+  cases h1;  case _ ts' fnf =>
+  cases fnf; case _ fnf ts' =>
+  cases ts'; have h := Val.app fnf n_stable;
+  simp at *;
+  have lem := classification_lemma fJ; simp at lem;
+  cases lem;
+  case _ h => cases h
+  case _ h =>
+    cases h; case _ k h =>
+    cases h; case _ k h =>
+    cases h; case _ aK bK =>
+    have arrK := Judgment.arrow aK bK;
+    have ih := ih1 h fJ arrK (ArrowLike.arrowt); cases ih;
+    case _ h =>
+      cases h;
+      case _ => cases fnf
+      case _ => cases fnf
+    case _ h =>
+      cases h;
+      case _ h =>
+        apply Or.inr; apply Or.inl;
+        unfold ValidHeadVariable;
+        have fanf := @Term.neutral_form_app f a ts'.1 ts'.2 fnf; symm at fanf;
+        apply Exists.intro (ts'.1, ts'.snd ++ [(.term, a)]);
+        apply And.intro; assumption; simp;
+        unfold ValidHeadVariable at h; simp at h;
+        cases h; case _ h => cases h; case _ fnf' h =>
+        rw [fnf] at fnf'; cases fnf'; case _ h =>
+        cases h; simp; assumption;
+      case _ h =>
+        apply Or.inr; apply Or.inr;
+        unfold ValidHeadVariable;
+        have fanf := @Term.neutral_form_app f a ts'.1 ts'.2 fnf; symm at fanf;
+        apply Exists.intro (ts'.1, ts'.snd ++ [(.term, a)]);
+        apply And.intro; assumption; simp;
+        unfold ValidHeadVariable at h; simp at h;
+        cases h; case _ h => cases h; case _ fnf' h =>
+        rw [fnf] at fnf'; cases fnf'; case _ h =>
+        cases h; simp; assumption;
+case _ ih1 _ =>
+  cases h1;
+  case _ h => cases h
+  case _ => constructor; constructor
+
+case _ Γ f A B a B' fJ aJ _ ih1 ih2 =>
+  cases h1; case _ n ts n_stable h1 =>
+  simp at h1; rw[Option.bind_eq_some] at h1;
+  cases h1;  case _ ts' fnf =>
+  cases fnf; case _ fnf ts' =>
+  cases ts'; have h := Val.app fnf n_stable;
+  simp at *;
+  have lem := classification_lemma fJ; simp at lem;
+  cases lem;
+  case _ h => cases h
+  case _ h =>
+    cases h; case _ k h =>
+    cases h; case _ k h =>
+    cases h; case _ aK bK =>
+    have arrK := Judgment.allt aK bK;
+    have ih := ih1 h fJ arrK (ArrowLike.allt); cases ih;
+    case _ h =>
+      cases h;
+      case _ => cases fnf
+      case _ => cases fnf
+    case _ h =>
+      cases h;
+      case _ h =>
+        apply Or.inr; apply Or.inl;
+        unfold ValidHeadVariable;
+        have fanf := @Term.neutral_form_appt f a ts'.1 ts'.2 fnf; symm at fanf;
+        apply Exists.intro (ts'.1, ts'.snd ++ [(.type, a)]);
+        apply And.intro; assumption; simp;
+        unfold ValidHeadVariable at h; simp at h;
+        cases h; case _ h => cases h; case _ fnf' h =>
+        rw [fnf] at fnf'; cases fnf'; case _ h =>
+        cases h; simp; assumption;
+      case _ h =>
+        apply Or.inr; apply Or.inr;
+        unfold ValidHeadVariable;
+        have fanf := @Term.neutral_form_appt f a ts'.1 ts'.2 fnf; symm at fanf;
+        apply Exists.intro (ts'.1, ts'.snd ++ [(.type, a)]);
+        apply And.intro; assumption; simp;
+        unfold ValidHeadVariable at h; simp at h;
+        cases h; case _ h => cases h; case _ fnf' h =>
+        rw [fnf] at fnf'; cases fnf'; case _ h =>
+        cases h; simp; assumption;
+case _ ih2 => cases h4
